pulse/share/steel/examples/pulse/lib/Pulse.Lib.Stick.fsti
@@ -43,3 +43,17 @@ val stick_sub_inv
 : stt_ghost unit emp_inames
     (stick #os1 hyp concl)
     (fun _ -> stick #os2 hyp concl)
+
+val ( forall* ) (#a:Type) (p:a->vprop) : vprop
+
+val elim_forall (#a:Type) (#p:a->vprop) (x:a)
+: stt_ghost unit emp_inames
+    (forall* x. p x)
+    (fun _ -> p x)
+
+val intro_forall (#a:Type) (#p:a->vprop)
+    (v:vprop)
+    (f_elim : (x:a -> stt_ghost unit emp_inames v (fun _ -> p x)))
+: stt_ghost unit emp_inames
+    v
+    (fun _ -> forall* x. p x)
